\documentclass{article}

\usepackage{amsmath}
\usepackage{mathtools}
\usepackage{extarrows}
\usepackage{bm}

\newcommand{\be}{\begin{equation}}
\newcommand{\ee}{\end{equation}}

\newcommand{\dif}{\,\mathrm{d}}
\newcommand{\p}{\partial}
\newcommand{\1}{\left}
\newcommand{\2}{\right}

\title{4-quantities in relativity}

\begin{document}
\maketitle

\section{Mehcnics}
\subsection*{Definitions}
4-velocity:
\be 
\begin{split}
U^a:=\1(\frac{\p}{\p\tau}\2)^a&=\frac{\dif t}{\dif\tau}\1(\frac{\p}{\p t}\2)^a+\frac{\dif x^i}{\dif \tau}\1(\frac{\p}{\p x^i}\2)^a\\
&=\gamma Z^a+h^a{}_b U^b
\end{split}
\ee
where $\gamma\equiv\dif t/\dif \tau=-U^a Z_a$, $Z^a\equiv(\p/\p t)^a$, and $h^a{}_b U^b$ is the space projection of $U^a$.\\

3-velocity:
\be 
u^a:=\frac{\dif x^i}{\dif t}\1(\frac{\p}{\p x^i}\2)^a=\frac{\dif x^i/\dif\tau}{\dif t/\dif\tau}\1(\frac{\p}{\p x^i}\2)^a=\frac{h^a{}_b U^b}{\gamma}.
\ee

So,
\be 
U^a=\gamma (Z^a+u^a)
\ee

4-momentum:
\be 
P^a:=mU^a=\gamma m Z^a+\gamma m u^a=E Z^a+p^a
\ee
where $E:=\gamma m=-P^aZ_a$ and $p^a:=\gamma m u^a$.\\

\be 
\1.
\begin{lgathered}
P^aP_a=mU^amU_a=-m^2\\
P^aP_a=(E Z^a+p^a)(E Z^a+p^a)=-E^2+p^2
\end{lgathered}
\2\}
\implies
E^2=m^2+p^2
\ee

4-acceleration:
\be 
A^a:=U^b\nabla_bU^a \implies A^aU_a=0\quad(\text{$A^a$ is orthogonal to $U^a$})
\ee
where $\nabla_a$ is the derivative operator compatible to the metric $g_{ab}$.\\

3-acceleration:
\be 
a^a:=\frac{\dif^2x^i}{\dif t^2}\1(\frac{\p}{\p x^i}\2)^a
\ee

4-force:
\be 
F^a:=U^b\nabla_bP^a=U^b\nabla_b(mU^a)\xlongequal{\text{if $m$=const}}mU^b\nabla_bU^a =mA^a
\ee

\section{Electromagnetics}
\subsection{Concepts}
4-wave vector:
\be 
K^a=\omega Z^a+k^a
\ee
where $\omega=-K^aZ_a$.

\be 
0=K^aK_a=(\omega Z^a+k^a)(\omega Z^a+k^a)=-\omega^2+k^2 \quad \implies \omega^2=k^2
\ee
\\
4-momentum of photons:
\be
P^a:=\hbar K^a=\hbar\omega Z^a+\hbar k^a=EZ^a+p^a
\ee
where
\be 
E=\hbar\omega, \qquad p^a=\hbar k^a
\ee
and
\be 
0=P^aP_a=(EZ^a+p^a)(EZ^a+p^a)=-E^2+p^2 \quad\implies E^2=p^2
 

\subsection{Gravitational redshift}
Let $\xi^a$ be the timelike killing vector of a stationary spacetime and $Z^a$ be a stationary observer,
\be 
\xi^a=\chi Z^a.
\ee

\be 
\xi^a\xi_a=\chi^2Z^aZ_a=-\chi^2 \quad \implies \chi=\sqrt{-\xi^a\xi_a}
\ee

\be 
\omega=-K^aZ_a=(-K^a\xi_a)\chi^{-1}
\ee

Due to the fact that $K^a$ is the tangent vector of null geodesics and $\xi^a$ is a killing vector, $(-K^a\xi_a)$ is a conservative quantity along the geodesics. Thus, 
\be 
\frac{\omega^\prime}{\omega}=\frac{\chi}{\chi^\prime} \quad\text{or}\quad \frac{\lambda^\prime}{\lambda}=\frac{\chi^\prime}{\chi}
\ee
so $\chi$ is called the \emph{redshift factor}.\\

In Schwarzschild spacetime,
\be 
\chi^2=-\xi^a\xi_a=-g_{ab}\1(\frac{\p}{\p t}\2)^a\1(\frac{\p}{\p t}\2)^b=-g_{00}=1-\frac{2M}{r}
\ee

\be 
\frac{\lambda^\prime}{\lambda}=\sqrt{\frac{1-2M/r^\prime}{1-2M/r}}
\ee
when $r^\prime>r$, $\lambda^\prime>\lambda$.
\end{document}