\documentclass{article}

\usepackage{amsmath}
\usepackage{mathtools}
\usepackage{extarrows}
\usepackage{bm}
\usepackage{geometry}
\geometry{centering,scale=0.8}

\newcommand{\be}{\begin{equation}}
\newcommand{\ee}{\end{equation}}
\newcommand{\bea}{\begin{eqnarray}}
\newcommand{\eea}{\end{eqnarray}}
\newcommand{\ba}{\begin{array}}
\newcommand{\ea}{\end{array}}

\newcommand{\dif}{\,\mathrm{d}}
\newcommand{\p}{\partial}
\newcommand{\1}{\left}
\newcommand{\2}{\right}

\title{Complex transformations}

\begin{document}
\maketitle

\section{Transformation from EF coordinate system}
\subsection{Ingoing coordinates with $``-"$ sign}
\be 
\begin{split}
\dif s^2&=-f\dif t^2-2\dif t\dif r+r^2\dif\Omega^2\\
&=-(1-\frac{2M}{r})\dif t^2-2\dif t\dif r+r^2\dif\Omega^2
\end{split}
\ee


\be
(g_{\mu\nu})=\left[\ba{cccc}-f&-1&0&0\\-1&0&0&0\\0&0&r^2&0\\0&0&0&r^2\sin^2\theta\ea\right]=\left[\ba{cccc}-(1-\frac{2M}{r})&-1&0&0\\-1&0&0&0\\0&0&r^2&0\\0&0&0&r^2\sin^2\theta\ea\right]
\ee

\be
(g^{\mu\nu})=\left[\ba{cccc}0&-1&0&0\\-1&f&0&0\\0&0&\frac 1 {r^2}&0\\0&0&0&\frac 1 {r^2\sin^2\theta}\ea\right]=\left[\ba{cccc}0&-1&0&0\\-1&(1-\frac{2M}{r})&0&0\\0&0&\frac 1 {r^2}&0\\0&0&0&\frac 1 {r^2\sin^2\theta}\ea\right]
\ee

\be
\begin{split}
g^{ab} =& g^{\mu\nu}\1(\frac \p {\p x^\mu}\2)^a\1(\frac \p {\p x^\nu}\2)^b\\
=& -\1(\frac \p {\p t}\2)^a\1(\frac \p {\p r}\2)^b-\1(\frac \p {\p r}\2)^a\1(\frac \p {\p t}\2)^b+\1(1-\frac{2M}{r}\2)\1(\frac \p {\p r}\2)^a\1(\frac \p {\p r}\2)^b \\
 & +\frac 1 {r^2} \1[\1(\frac \p {\p\theta}\2)^a \1(\frac \p {\p\theta}\2)^b+\frac 1 {\sin^2 \theta} \1(\frac \p {\p\phi}\2)^a \1(\frac \p {\p\phi}\2)^b \2] 
\end{split}
\ee

\be
\1\{
\begin{split}
l^a&\equiv \1(\frac \p {\p r}\2)^a\\
k^a&\equiv \1(\frac \p {\p t}\2)^a-\frac 1 2 \1(1-\frac{2M}{r}\2)\1(\frac \p {\p r}\2)^a\\
m^a&\equiv \frac 1 {\sqrt 2 r}\1[\1(\frac \p {\p\theta}\2)^a+\frac i {\sin\theta} \1(\frac \p {\p\phi}\2)^a\2]
\end{split}
\2.
\ee

\be
g^{ab}=-l^ak^b-l^bk^a+m^a{\bar m}^b+m^b{\bar m}^a
\ee

Assume $r$ and $t$ to be complex so that they can be divided into real and imaginary part, (while $\theta$ and $\phi$ remains real,)
\be
\1\{
\begin{split}
r&=R+iacos\Theta\\
t&=T-iacos\Theta\\
\theta&=\Theta\\
\phi&=\Phi
\end{split}
\2.
\ee

\be
\1\{
\begin{split}
\1(\frac \p {\p R}\2)^a&=\1(\frac \p {\p r}\2)^a\\
\1(\frac \p {\p T}\2)^a&=\1(\frac \p {\p t}\2)^a\\
\1(\frac \p {\p \Theta}\2)^a&=\1(\frac \p {\p \theta}\2)^a-ia\sin\theta\1(\frac \p {\p r}\2)^a+ia\sin\theta\1(\frac \p {\p t}\2)^a\\
\1(\frac \p {\p \Phi}\2)^a&=\1(\frac \p {\p \phi}\2)^a
\end{split}
\2.
\ee

\be
\begin{split}
\frac 2 r \rightarrow Re\1(\frac 2 r\2)&=\frac 1 r+\frac 1 {\bar r}\\
&=\frac 1 {R+iacos\Theta}+\frac 1 {R-iacos\Theta}\\
&=\frac{2R}{{R}^2+a^2 cos^2 \Theta}\\
&\equiv \frac{2R}{\rho^2}
\end{split}
\ee

\be
\frac 1 {r^2} \rightarrow \frac 1 {r \bar r}=\frac{1}{(R+iacos\Theta)(R-iacos\Theta)}=\frac{1}{{R}^2+a^2 cos^2 \Theta}=\frac{1}{\rho^2}
\ee

So, in $(t,R,\theta,\phi)$:
\be
\1\{
\begin{split}
{l^\prime}^a&\equiv \1(\frac \p {\p R}\2)^a\\
{k^\prime}^a&\equiv \1(\frac \p {\p T}\2)^a-\frac 1 2 \1(1-\frac{2MR}{\rho^2}\2)\1(\frac \p {\p R}\2)^a\\
&=\1(\frac \p {\p t}\2)^a-\frac 1 2 \1(1-\frac{2MR}{\rho^2}\2)\1(\frac \p {\p R}\2)^a\\
{m^\prime}^a&\equiv \frac 1 {\sqrt 2 \bar r}\1[\1(\frac \p {\p\Theta}\2)^a+\frac i {\sin\Theta} \1(\frac \p {\p\Phi}\2)^a\2]\\
&=\frac 1 {\sqrt 2 \bar r}\1[\1(\frac \p {\p \theta}\2)^a-ia\sin\theta\1(\frac \p {\p r}\2)^a+ia\sin\theta\1(\frac \p {\p t}\2)^a+\frac i {\sin\theta} \1(\frac \p {\p\phi}\2)^a\2]\\
&=\frac 1 {\sqrt 2 \bar r}\1[\1(\frac \p {\p \theta}\2)^a-ia\sin\theta\1(\frac \p {\p R}\2)^a+ia\sin\theta\1(\frac \p {\p t}\2)^a+\frac i {\sin\theta} \1(\frac \p {\p\phi}\2)^a\2]\\
{\bar m}^{\prime a}
&=\frac 1 {\sqrt 2 r}\1[\1(\frac \p {\p \theta}\2)^a+ia\sin\theta\1(\frac \p {\p R}\2)^a-ia\sin\theta\1(\frac \p {\p t}\2)^a-\frac i {\sin\theta} \1(\frac \p {\p\phi}\2)^a\2]
\end{split}
\2.
\ee

\be
g^{\prime ab}=-l^{\prime a}k^{\prime b}-l^{\prime b}k^{\prime a}+m^{\prime a}{\bar m}^{\prime b}+m^{\prime b}{\bar m}^{\prime a}
\ee

\newpage

\be 
-l^{\prime a}k^{\prime b}-l^{\prime b}k^{\prime a}
=-\1(\frac \p {\p t}\2)^a\1(\frac \p {\p r}\2)^b-\1(\frac \p {\p r}\2)^a\1(\frac \p {\p t}\2)^b+\1(1-\frac{2MR}{\rho^2}\2)\1(\frac \p {\p R}\2)^a\1(\frac \p {\p R}\2)^b
\ee

\be 
m^{\prime a}{\bar m}^{\prime b}+m^{\prime b}{\bar m}^{\prime a}=\frac{1}{\rho^2}
\1\{
\begin{split}
& \1(\frac \p {\p \theta}\2)^a\1(\frac \p {\p \theta}\2)^b+a^2\sin^2\theta\1(\frac \p {\p R}\2)^a\1(\frac \p {\p R}\2)^b+a^2\sin^2\theta\1(\frac \p {\p t}\2)^a\1(\frac \p {\p t}\2)^b+\frac{1}{\sin^2\theta}\1(\frac \p {\p \phi}\2)^a\1(\frac \p {\p \phi}\2)^b\\
&-a^2\sin^2\theta\1(\frac \p {\p t}\2)^a\1(\frac \p {\p R}\2)^b-a^2\sin^2\theta\1(\frac \p {\p R}\2)^a\1(\frac \p {\p t}\2)^b\\
&+a\1(\frac \p {\p t}\2)^a\1(\frac \p {\p \phi}\2)^b+a\1(\frac \p {\p \phi}\2)^a\1(\frac \p {\p t}\2)^b \\
&-a\1(\frac \p {\p R}\2)^a\1(\frac \p {\p \phi}\2)^b-a\1(\frac \p {\p \phi}\2)^a\1(\frac \p {\p R}\2)^b
\end{split}
\2.
\ee

\be 
\1\{
\begin{split}
g^{tt}&=\frac{a^2\sin^2\theta}{\rho^2}\\
g^{R R}&=1-\frac{2MR}{\rho^2}+\frac{a^2\sin^2\theta}{\rho^2}=\frac{R^2+a^2-2MR}{\rho^2}\\
g^{\theta\theta}&=\frac{1}{\rho^2}\\
g^{\phi\phi}&=\frac{1}{\rho^2 \sin^2\theta}
\end{split}
\2.
\ee

\be 
\1\{
\begin{split}
g^{tR}&=g^{Rt}=-1-\frac{a^2\sin^2\theta}{\rho^2}=-\frac{(R^2+a^2)}{\rho^2}\\
g^{t\phi}&=g^{\phi T}=\frac{a}{\rho^2}\\
g^{R\phi}&=g^{\phi R}=-\frac{a}{\rho^2}\\
\end{split}
\2.
\ee

\be
(g^{\prime\mu\nu})=\frac{1}{\rho^2}\left[\ba{cccc}a^2\sin^2\theta&-(R^2+a^2)&0&a\\ \noalign{\medskip}-(R^2+a^2)&R^2+a^2-2MR&0&-a\\ \noalign{\medskip}0&0&1&0\\ \noalign{\medskip}a&-a&0&\frac 1 {\sin^2\theta}\ea\right]
\ee

\be 
(g^\prime_{\mu\nu})=\left[ \begin {array}{cccc} -(1-\,{\frac {2MR}{{\rho}^{2}}})&-1&0&-\,{
\frac {2MRa{\sin}^{2}\theta}{{\rho}^{2}}}\\ \noalign{\medskip}-1&0&0&
a\,{\sin}^{2}\theta\\ \noalign{\medskip}0&0&{\rho}^{2}&0
\\ \noalign{\medskip}-\,{\frac {2MRa{\sin}^{2}\theta}{{\rho}^{2}}}&
a\,{\sin}^{2}\theta&0& \left( {R}^{2}+{a}^{2} \right) {\sin}^{2}\theta
+\,{\frac {2MR{a}^{2}{\sin}^{4}\theta}{{\rho}^{2}}}\end {array}
 \right] 
\ee

\be 
\dif s^2=-(1-\,{\frac {2MR}{{\rho}^{2}}})\dif t^2-2\dif t \dif R-\,{
\frac {2MR}{{\rho}^{2}}}(2a{\sin}^{2}\theta)\dif t\dif\phi +2a\sin^2\theta \dif R\dif\phi+\rho^2\dif \theta^2+\1[(R^2+a^2)\sin^2\theta+\frac{2MR}{\rho^2}(a^2\sin^4\theta)\2]\dif\phi^2
\ee

\subsection{Outgoing coordinates with $``+"$ sign}

\newpage
\section{transformation from PG coordinate system}
\subsection{Ingoing coordinates}

\be
\begin{split}
\mathrm ds^2&=-f\mathrm dt^2-2\sqrt{1-f}\mathrm dt\mathrm dr+\mathrm dr^2+r^2\mathrm d\Omega^2\\
&=- \mathrm dt^2+(\mathrm dr- \sqrt{1-f}\mathrm dt)^2+r^2\mathrm d\Omega^2,
\end{split}
\ee

\be
\begin{split}
\mathrm ds^2&=-(1-\frac{2M}{r})\mathrm dt^2-2\sqrt{\frac{2M}{r}}\mathrm dt\mathrm dr+\mathrm dr^2+r^2\mathrm d\Omega^2\\
&=- \mathrm dt^2+(\mathrm dr- \sqrt{\frac{2M}{r}}\mathrm dt)^2+r^2\mathrm d\Omega^2,
\end{split}
\ee

\be
(g_{\mu\nu})=\left[\ba{cccc}-f&-\sqrt{1-f}&0&0\\-\sqrt{1-f}&1&0&0\\0&0&r^2&0\\0&0&0&r^2\sin^2\theta\ea\right]=\left[\ba{cccc}-(1-\frac{2M}{r})&-\sqrt{\frac{2M}{r}}&0&0\\-\sqrt{\frac{2M}{r}}&1&0&0\\0&0&r^2&0\\0&0&0&r^2\sin^2\theta\ea\right]
\ee

\be
(g^{\mu\nu})=\left[\ba{cccc}-1&-\sqrt{1-f}&0&0\\-\sqrt{1-f}&f&0&0\\0&0&\frac 1 {r^2}&0\\0&0&0&\frac 1 {r^2\sin^2\theta}\ea\right]=\left[\ba{cccc}-1&-\sqrt{\frac{2M}{r}}&0&0\\-\sqrt{\frac{2M}{r}}&(1-\frac{2M}{r})&0&0\\0&0&\frac 1 {r^2}&0\\0&0&0&\frac 1 {r^2\sin^2\theta}\ea\right]
\ee

\be
\begin{split}
g^{ab} =& g^{\mu\nu}\1(\frac \p {\p x^\mu}\2)^a\1(\frac \p {\p x^\nu}\2)^b\\
=& -\1(\frac \p {\p t}\2)^a\1(\frac \p {\p t}\2)^b-\sqrt{1-f}\1(\frac \p {\p t}\2)^a\1(\frac \p {\p r}\2)^b-\sqrt{1-f}\1(\frac \p {\p r}\2)^a\1(\frac \p {\p t}\2)^b+f\1(\frac \p {\p r}\2)^a\1(\frac \p {\p r}\2)^b \\
 & +\frac 1 {r^2} \1[\1(\frac \p {\p\theta}\2)^a \1(\frac \p {\p\theta}\2)^b+\frac 1 {\sin^2 \theta} \1(\frac \p {\p\phi}\2)^a \1(\frac \p {\p\phi}\2)^b \2] \\
=& -\1(\frac \p {\p t}\2)^a\1(\frac \p {\p t}\2)^b-\sqrt{\frac{2M}{r}}\1(\frac \p {\p t}\2)^a\1(\frac \p {\p r}\2)^b-\sqrt{\frac{2M}{r}}\1(\frac \p {\p r}\2)^a\1(\frac \p {\p t}\2)^b+\1(1-\frac{2M}{r}\2)\1(\frac \p {\p r}\2)^a\1(\frac \p {\p r}\2)^b \\
 & +\frac 1 {r^2} \1[\1(\frac \p {\p\theta}\2)^a \1(\frac \p {\p\theta}\2)^b+\frac 1 {\sin^2 \theta} \1(\frac \p {\p\phi}\2)^a \1(\frac \p {\p\phi}\2)^b \2]
\end{split}
\ee 

After complexifying,

\be
\1\{ 
\begin{split}
g^{tt}&=-1+\frac{a^2\sin^2\theta}{\rho^2}=\frac{1}{\rho^2}(a^2\sin^2\theta-\rho^2)\\
g^{tR}&=g^{Rt}=-\sqrt{\frac{2Mr}{\rho^2}}-\frac{a^2\sin^2\theta}{\rho^2}=-\frac{1}{\rho^2}(a^2\sin^2\theta+\sqrt{2Mr\rho^2})
\end{split}
\2.
\ee

\be
(g^{\prime\mu\nu})=\frac{1}{\rho^2}\left[\ba{cccc}a^2\sin^2\theta-\rho^2&-(a^2\sin^2\theta+\sqrt{2Mr\rho^2})&0&a\\ \noalign{\medskip}-(a^2\sin^2\theta+\sqrt{2Mr\rho^2})&R^2+a^2-2Mr&0&-a\\ \noalign{\medskip}0&0&1&0\\ \noalign{\medskip}a&-a&0&\frac 1 {\sin^2\theta}\ea\right]
\ee

\be 
(g^\prime_{\mu\nu})=\left[ \begin {array}{cccc} -\1(1-\,{\frac {2Mr}{{\rho}^{2}}}\2)&-\sqrt{\frac{2Mr}{\rho^2}}&0&\1(1-\frac{2Mr}{\rho^2}-\sqrt{\frac{2Mr}{\rho^2}}\2)a\sin^2\theta\\ \noalign{\medskip}-\sqrt{\frac{2Mr}{\rho^2}}&1&0&
\1(1+\sqrt{\frac{2Mr}{\rho^2}}\2)a\,{\sin}^{2}\theta\\ \noalign{\medskip}0&0&{\rho}^{2}&0
\\ \noalign{\medskip}\1(1-\frac{2Mr}{\rho^2}-\sqrt{\frac{2Mr}{\rho^2}}\2)a\sin^2\theta&
\1(1+\sqrt{\frac{2Mr}{\rho^2}}\2)a\,{\sin}^{2}\theta&0& \left( {r}^{2}+{a}^{2} \right) {\sin}^{2}\theta
-\1(1-\frac{2Mr}{\rho^2}-\sqrt{\frac{2Mr}{\rho^2}}\2)a^2\sin^4\theta\end {array}
 \right] 
\ee

\subsection{Outgoing coordinates}


\newpage
\section{transformation from PG-like coordinate system}
\subsection{Ingoing coordinates}

\be
\begin{split}
\mathrm ds^2&=-f\mathrm dt^2-2\sqrt{1-pf}\mathrm dt\mathrm dr+p\mathrm dr^2+r^2\mathrm d\Omega^2\\
&=-\frac 1 p \mathrm dt^2+p(\mathrm dr-\frac 1 p \sqrt{1-pf}\mathrm dt)^2+r^2\mathrm d\Omega^2,
\end{split}
\ee

\be
(g_{\mu\nu})=\left[\ba{cccc}-f&-\sqrt{1-pf}&0&0\\-\sqrt{1-pf}&p&0&0\\0&0&r^2&0\\0&0&0&r^2\sin^2\theta\ea\right]
\ee

\be
(g^{\mu\nu})=\left[\ba{cccc}-p&-\sqrt{1-pf}&0&0\\-\sqrt{1-pf}&f&0&0\\0&0&\frac 1 {r^2}&0\\0&0&0&\frac 1 {r^2\sin^2\theta}\ea\right]
\ee

\be
\begin{split}
g^{ab} =& g^{\mu\nu}\1(\frac \p {\p x^\mu}\2)^a\1(\frac \p {\p x^\nu}\2)^b\\
=& -p\1(\frac \p {\p t}\2)^a\1(\frac \p {\p t}\2)^b-\sqrt{1-pf}\1(\frac \p {\p t}\2)^a\1(\frac \p {\p r}\2)^b-\sqrt{1-pf}\1(\frac \p {\p r}\2)^a\1(\frac \p {\p t}\2)^b+f\1(\frac \p {\p r}\2)^a\1(\frac \p {\p r}\2)^b \\
 & +\frac 1 {r^2} \1[\1(\frac \p {\p\theta}\2)^a \1(\frac \p {\p\theta}\2)^b+\frac 1 {\sin^2 \theta} \1(\frac \p {\p\phi}\2)^a \1(\frac \p {\p\phi}\2)^b \2] 
\end{split}
\ee 

After complexifying,

\be
\1\{ 
\begin{split}
g^{tt}&=-p+\frac{a^2\sin^2\theta}{\rho^2}=\frac{1}{\rho^2}(a^2\sin^2\theta-p\rho^2)\\
g^{tR}&=g^{Rt}=-\sqrt{1-pf}-\frac{a^2\sin^2\theta}{\rho^2}=-\frac{1}{\rho^2}(a^2\sin^2\theta+\rho^2\sqrt{1-pf})
\end{split}
\2.
\ee

\be
(g^{\prime\mu\nu})=\frac{1}{\rho^2}\left[\ba{cccc}a^2\sin^2\theta-p\rho^2&-(a^2\sin^2\theta+\rho^2\sqrt{1-pf})&0&a\\ \noalign{\medskip}-(a^2\sin^2\theta+\rho^2\sqrt{1-pf})&R^2+a^2-2Mr&0&-a\\ \noalign{\medskip}0&0&1&0\\ \noalign{\medskip}a&-a&0&\frac 1 {\sin^2\theta}\ea\right]
\ee

\subsection{Outgoing coordinates}

\end{document}