\documentclass{article}

\usepackage{amsmath,bm}

\newcommand{\be}{\begin{equation}}
\newcommand{\ee}{\end{equation}}

\title{Green's function in Quantum Scattering Problem}
\author{}
\date{}

\begin{document}
\maketitle

\section{Generating Green's function}
Schrodinger's equation:
\be
i\hbar\frac{\partial}{\partial t}\psi=\hat{H}\psi
\ee
ding tai:
\be
E\psi=\hat H\psi=(\frac{p^2}{2m}+V)\psi=(-\frac{\hbar^2}{2m}\nabla^2+V)\psi
\ee
In 3-dimensional coordinate biao xiangï¼š
\be
(\nabla^2+k^2)\psi(\vec{r})=\frac{2\mu}{\hbar^2}V(r)\psi(\vec{r})
\label{3D}
\ee
The right-hand side:
\be
\frac{2\mu}{\hbar^2}V(r)\psi(\vec{r})=\frac{2\mu}{\hbar^2}\int \delta(\vec{r}-\vec{r}')V(r')\psi(\vec{r}') d\vec{r}' 
\label{righthand}
\ee
Here we assume
\be
\psi(\vec{r})=\frac{2\mu}{\hbar^2}\int G(\vec{r},\vec{r}')V(r')\psi(\vec{r}') d\vec{r}' 
\label{assume}
\ee
Thus we bring (\ref{assume}) and (\ref{righthand}) into (\ref{3D}), we get
\be
\boxed{\bm{(\nabla^2+k^2)G(\vec{r},\vec{r}')=\delta(\vec{r}-\vec{r}')}}
\label{Green}
\ee
The general form of $\psi(\vec{r})$ can be written as
\be
\psi(\vec{r})=\psi_i(\vec{r})+\frac{2\mu}{\hbar^2}\int G(\vec{r},\vec{r}')V(r')\psi(\vec{r}') d\vec{r}' 
\ee
where $\psi_i(\vec{r})$ satisfies
\be
(\nabla^2+k^2)\psi_i(\vec{r})=0
\ee
In scattering problem we choose $\psi_i(\vec{r})=e^{ikz}$, so
\be
\psi(\vec{r})=e^{ikz}+\frac{2\mu}{\hbar^2}\int G(\vec{r},\vec{r}')V(r')\psi(\vec{r}') d\vec{r}'
\ee
\section{Solving Green's function}
\subsection{Fourier's transformation}
In order to solve equation(\ref{Green}), we execute Fourier's transformation first,
\be
G(\vec{r}-\vec{r}')=\int \tilde{G}(\vec{q}) e^{i\vec{q}(\vec{r}-\vec{r}')} d^3 q
\label{Fourier}
\ee
then we bring it into (\ref{Green}), we get
\be
\int (\nabla^2+k^2) e^{i\vec{q}(\vec{r}-\vec{r}')} \tilde{G}(\vec{q}) d^3 q=\delta(\vec{r}-\vec{r}')
\ee
i.e.
\be
\int (-q^2+k^2) e^{i\vec{q}(\vec{r}-\vec{r}')} \tilde{G}(\vec{q}) d^3 q=\frac{1}{(2\pi)^3}\int e^{i\vec{q}(\vec{r}-\vec{r}')}  d^3 q
\ee
So we have
\be
\fbox{$\displaystyle{\tilde{G}(\vec{q})=\frac{1}{(2\pi)^3}\frac{1}{(-q^2+k^2)}}$}
\ee
Bringing this into (\ref{Fourier}), we have
\be
G(\vec{r}-\vec{r}')=-\frac{1}{(2\pi)^3}\int e^{i\vec{q}(\vec{r}-\vec{r}')} \frac{1}{(q^2-k^2)} d^3 q
\ee
\subsection{Complex integral}

\end{document}
